Reprove properties of the retransmit model

fairneris/examples/retransmit_model.v
@@ -1,7 +1,7 @@
 From trillium.prelude Require Export finitary quantifiers sigma classical_instances.
 From Paco Require Import paco1 paco2 pacotac.
 From fairneris Require Export trace_utils fairness env_model.
-From fairneris.aneris_lang Require Import ast network lang aneris_lang.
+From fairneris.aneris_lang Require Import ast network lang aneris_lang adequacy network_model.
 From fairneris Require Export trace_utils ltl_lite.
 
 Import derived_laws_later.bi.
@@ -70,7 +70,7 @@ Inductive retransmit_trans :
 | B_SendDone :
   retransmit_trans Received (Brole, Some (Send mDone)) Done
 .
-Notation mtrace := (trace retransmit_state (retransmit_role * option aneris_action)).
+
 
 Definition retransmit_live_roles (s : retransmit_state) : gset retransmit_role :=
   {[Arole]} ∪
@@ -83,81 +83,51 @@ Lemma retransmit_live_spec_holds s ρ α s' :
   retransmit_trans s (ρ,α) s' → ρ ∈ retransmit_live_roles s.
 Proof. inversion 1; set_solver. Qed.
 
-Definition send_filter msg : retransmit_label → Prop :=
-  λ l, snd l = Some $ Send msg.
-Instance send_filter_decision msg l : Decision (send_filter msg l).
-Proof. apply make_decision. Qed.
+Definition retransmit_lts : Lts (retransmit_role * option (action aneris_lang)) :=
+  {|
+            lts_state := retransmit_state;
+            lts_trans := retransmit_trans;
+  |}.
 
-Definition recv_filter msg : retransmit_label → Prop :=
-  λ l, snd l = Some $ Recv (m_destination msg) (Some msg).
-Instance recv_filter_decision msg l : Decision (recv_filter msg l).
-Proof. apply make_decision. Qed.
-
-Definition any_recv_filter sa : retransmit_label → Prop :=
-  λ l, exists rcv, snd l = Some $ Recv sa rcv.
-Instance any_recv_filter_decision l sa : Decision (any_recv_filter sa l).
-Proof. apply make_decision. Qed.
-
-Definition retransmit_fair_network_delivery msg : mtrace → Prop :=
-  □ (□◊ℓ↓send_filter msg → □◊ℓ↓ any_recv_filter (m_destination msg) → ◊ℓ↓ recv_filter msg).
-
-Definition retransmit_fair_network (mtr : mtrace) : Prop :=
-  ∀ msg, retransmit_fair_network_delivery msg mtr.
-
-(* TODO: This should be generalised, and lifted to multiple roles *)
-Definition retransmit_terminating_role (ρ : retransmit_role) (tr : mtrace) : Prop :=
-  (◊↓λ st _, ρ ∉ retransmit_live_roles st) tr ∨ ¬ infinite_trace tr.
-
-Definition retransmit_fair_scheduling_mtr (ρ : retransmit_role) : mtrace → Prop :=
-  trace_always_eventually_implies_now
-    (λ δ _, retransmit_role_enabled_model ρ δ)
-    (λ δ (ℓ: option retransmit_label), ¬ retransmit_role_enabled_model ρ δ ∨
-              option_map fst ℓ = Some ρ).
-
-Definition retransmit_fair_scheduling (mtr : mtrace) : Prop :=
-  ∀ ρ, retransmit_fair_scheduling_mtr ρ mtr.
-
-Definition mtrace_fair (mtr : mtrace) : Prop :=
-  retransmit_fair_scheduling mtr ∧ retransmit_fair_network mtr.
-
-Lemma mtrace_fair_always mtr :
-  mtrace_fair mtr ↔ (□ mtrace_fair) mtr.
+Definition retransmit_model : UserModel aneris_lang.
 Proof.
+  refine({|
+            usr_role := retransmit_role;
+            usr_lts := retransmit_lts;
+            usr_live_roles := retransmit_live_roles;
+            usr_live_spec := retransmit_live_spec_holds;
+            usr_fl _ := 20;
+          |}).
+Defined.
+
+Notation mtrace := (lts_trace retransmit_model).
+
+(* Put somewhere *)
+Lemma mtrace_fair_always (mtr : mtrace) :
+  usr_fair mtr ↔ (□ usr_fair) mtr.
+Proof.
+  split; last by intros Hfair%trace_always_elim.
+  rewrite /usr_fair /usr_network_fair_send_receive /usr_network_fair_send_receive_of
+    /usr_fair_scheduling /usr_fair_scheduling_mtr.
+  intros [Hmtr1 Hmtr2].
+  apply trace_always_forall in Hmtr1.
+  apply trace_always_forall in Hmtr2.
+  eassert ((□ trace_and _ _) mtr).
+  { apply trace_always_and. split; [apply Hmtr1|apply Hmtr2]. }
+  apply trace_always_idemp in H.
+  revert H. apply trace_always_mono.
+  intros tr.
+  apply trace_impliesI.
+  intros Htr.
+  apply trace_always_and in Htr as [Htr1 Htr2].
   split.
-  - rewrite /mtrace_fair.
-    intros [Hmtr1 Hmtr2].
-    rewrite /retransmit_fair_scheduling in Hmtr1.
-    rewrite /retransmit_fair_network in Hmtr2.
-    rewrite /retransmit_fair_scheduling_mtr in Hmtr1.
-    rewrite /retransmit_fair_network_delivery in Hmtr2.
-    apply trace_always_forall in Hmtr1.
-    apply trace_always_forall in Hmtr2.
-    eassert ((□ trace_and _ _) mtr).
-    { apply trace_always_and. split; [apply Hmtr1|apply Hmtr2]. }
-    apply trace_always_idemp in H.
-    revert H. apply trace_always_mono.
-    intros tr.
-    apply trace_impliesI.
-    intros Htr.
-    apply trace_always_and in Htr as [Htr1 Htr2].
-    split.
-    + intros x. revert Htr1.
-      apply trace_always_mono. intros tr'. apply trace_impliesI.
-      intros Htr'. done.
-    + intros x. revert Htr2.
-      apply trace_always_mono. intros tr'. apply trace_impliesI.
-      intros Htr'. done.
-  - by intros Hfair%trace_always_elim.
+  + intros x. revert Htr1.
+    apply trace_always_mono. intros tr'. apply trace_impliesI.
+    intros Htr'. done.
+  + intros x. revert Htr2.
+    apply trace_always_mono. intros tr'. apply trace_impliesI.
+    intros Htr'. done.
 Qed.
-
-Definition trans_valid (mtr : mtrace) :=
-   match mtr with
-   | ⟨s⟩ => True
-   | (s -[l]-> tr) => retransmit_trans s l (trfirst tr)
-   end.
-
-Definition mtrace_valid (mtr : mtrace) :=
-  trace_always trans_valid mtr.
 
 Definition option_lift {S L} (P : S → L → Prop) : S → option L → Prop :=
   λ s ol, ∃ l, ol = Some l ∧ P s l.
@@ -173,43 +143,45 @@ Proof. apply trace_always_universal.
   by destruct mtr'; set_solver.
 Qed.
 
-Lemma B_always_live_infinite (mtr : mtrace) :
-  ¬ retransmit_terminating_role Brole mtr →
-  (□ (trace_now (λ s _, retransmit_role_enabled_model Brole s))) mtr.
-Proof.
-  intros Hnt. apply trace_alwaysI. intros mtr' Hsuff.
-  rewrite /trace_now /pred_at /retransmit_role_enabled_model.
-  have ? : Brole ∈ retransmit_live_roles (trfirst mtr'); last destruct mtr' =>//=.
-  apply NNP_P => Hin. apply Hnt.
-  rewrite /retransmit_terminating_role. left.
-  eapply (trace_eventually_suffix_of _ mtr') =>//. apply trace_eventually_intro.
-  by destruct mtr'.
-Qed.
+(* Lemma B_always_live_infinite (mtr : mtrace) : *)
+(*   ¬ retransmit_terminating_role Brole mtr → *)
+(*   (□ (trace_now (λ s _, retransmit_role_enabled_model Brole s))) mtr. *)
+(* Proof. *)
+(*   intros Hnt. apply trace_alwaysI. intros mtr' Hsuff. *)
+(*   rewrite /trace_now /pred_at /retransmit_role_enabled_model. *)
+(*   have ? : Brole ∈ retransmit_live_roles (trfirst mtr'); last destruct mtr' =>//=. *)
+(*   apply NNP_P => Hin. apply Hnt. *)
+(*   rewrite /retransmit_terminating_role. left. *)
+(*   eapply (trace_eventually_suffix_of _ mtr') =>//. apply trace_eventually_intro. *)
+(*   by destruct mtr'. *)
+(* Qed. *)
 
 Lemma B_always_live_always_eventually_receive (mtr : mtrace) :
-  mtrace_fair mtr →
-  mtrace_valid mtr →
+  usr_fair mtr →
+  usr_trace_valid mtr →
   (□ (trace_now (λ s _, s = Start))) mtr →
-  (□◊ℓ↓ any_recv_filter saB) mtr.
+  (□◊ℓ↓ usr_any_recv_filter saB) mtr.
 Proof.
   intros Hf Hval Hae. apply trace_alwaysI. intros mtr' Hsuff.
-  have Hfs': retransmit_fair_scheduling mtr'.
-  { by apply mtrace_fair_always, (trace_always_suffix_of _ _ _ Hsuff), trace_always_elim in Hf as [??]. }
-  rewrite /retransmit_fair_scheduling in Hfs'.
-  specialize (Hfs' Brole).
-  rewrite /retransmit_fair_scheduling_mtr in Hfs'.
-  rewrite /trace_always_eventually_implies_now in Hfs'.
-  rewrite /trace_always_eventually_implies in Hfs'.
-  have He: (↓ λ s _, s = Start) mtr'.
-  { apply trace_always_elim in Hfs'.
-    apply (trace_always_suffix_of _ _ _ Hsuff) in Hae.
-    by apply trace_always_elim in Hae. }
-  have He': (↓ λ s _, retransmit_role_enabled_model Brole s) mtr'.
-  { eapply trace_now_mono=>//. move=> s l /= ->.
-    rewrite /retransmit_role_enabled_model. set_solver. }
-  apply trace_always_elim in Hfs'.
-  rewrite trace_impliesI in Hfs'.
-  specialize (Hfs' He'). clear He'.
+  (* have Hfs': retransmit_fair_scheduling mtr'. *)
+  (* { by apply mtrace_fair_always, (trace_always_suffix_of _ _ _ Hsuff), trace_always_elim in Hf as [??]. } *)
+  (* rewrite /retransmit_fair_scheduling in Hfs'. *)
+  (* specialize (Hfs' Brole). *)
+  (* rewrite /retransmit_fair_scheduling_mtr in Hfs'. *)
+  (* rewrite /trace_always_eventually_implies_now in Hfs'. *)
+  (* rewrite /trace_always_eventually_implies in Hfs'. *)
+  (* have He: (↓ λ s _, s = Start) mtr'. *)
+  (* { apply trace_always_elim in Hfs'. *)
+  (*   apply (trace_always_suffix_of _ _ _ Hsuff) in Hae. *)
+  (*   by apply trace_always_elim in Hae. } *)
+  (* have He': (↓ λ s _, retransmit_role_enabled_model Brole s) mtr'. *)
+  (* { eapply trace_now_mono=>//. move=> s l /= ->. *)
+  (*   rewrite /retransmit_role_enabled_model. set_solver. } *)
+  (* apply trace_always_elim in Hfs'. *)
+  (* rewrite trace_impliesI in Hfs'. *)
+  (* specialize (Hfs' He'). clear He'. *)
+
+
   (* apply trace_eventuallyI in Hfs' as (mtr'' & Hsuff' & Hfs''). *)
   (* apply (trace_eventually_suffix_of _ mtr'') =>//. *)
   (* have Hsuff2: trace_suffix_of mtr'' mtr by eapply trace_suffix_of_trans. *)
@@ -251,32 +223,43 @@ Admitted.
 (*     rewrite /retransmit_role_enabled_model in Htr. set_solver. *)
 (* Qed. *)
 
-(* Lemma retransmit_fair_traces_eventually_mAB mtr : *)
-(*   mtrace_valid mtr → retransmit_fair_scheduling_mtr Arole mtr → *)
-(*   (◊ ℓ↓ send_filter mAB) mtr. *)
-(* Proof. *)
-(*   intros Hvalid Hfair. *)
-(*   pose proof (retransmit_fair_traces_eventually_A mtr Hfair) as Htr. *)
-(*   eapply trace_eventually_mono_strong; [|done]. *)
-(*   intros tr' Htr'. *)
-(*   eapply trace_always_suffix_of in Hvalid; [|done]. *)
-(*   apply trace_always_elim in Hvalid. *)
-(*   destruct tr' as [s|s l tr']; [done|]. *)
-(*   apply trace_now_mono_strong. *)
-(*   intros ???? HP; simplify_eq. *)
-(*   destruct l. destruct r=>//. simpl in *. *)
-(*   simplify_eq. inversion Hvalid. inversion H1. by simplify_eq. *)
-(* Qed. *)
+Lemma retransmit_fair_traces_eventually_mAB (mtr : mtrace) :
+  usr_trace_valid mtr → usr_fair mtr →
+  (◊ ℓ↓ usr_send_filter mAB) mtr.
+Proof.
+  intros Hvalid [Hfairn Hfairs].
+  specialize (Hfairs Arole).
+  rewrite /usr_fair_scheduling_mtr in Hfairs.
 
-(* Lemma retransmit_fair_traces_always_eventually_mAB mtr : *)
-(*   mtrace_valid mtr → retransmit_fair_scheduling_mtr Arole mtr → *)
-(*   (□ ◊ ℓ↓ send_filter mAB) mtr. *)
-(* Proof. *)
-(*   intros Hvalid Hfair. eapply trace_always_implies_always; *)
-(*     [|apply trace_always_and; split; [apply Hvalid|apply Hfair]]. *)
-(*   intros tr' [Hvalid' Hfair']%trace_always_and. *)
-(*   by apply retransmit_fair_traces_eventually_mAB. *)
-(* Qed. *)
+  apply trace_always_elim in Hfairs.
+  rewrite trace_impliesI in Hfairs.
+  ospecialize (Hfairs _).
+  { rewrite /trace_now /pred_at /=. destruct mtr; simpl; set_solver. }
+
+  eapply trace_eventually_mono_strong; last apply Hfairs.
+  intros tr Hsuff Htr.
+  rewrite /trace_now /pred_at /= in Htr *.
+  destruct tr; simpl.
+  { exfalso. destruct Htr; [set_solver | naive_solver]. }
+  destruct Htr as [|[act Htr]]; [set_solver |]. simplify_eq.
+  eapply trace_always_suffix_of in Hvalid=>//.
+  eapply trace_always_elim in Hvalid.
+  inversion Hvalid; simplify_eq.
+  rewrite /trace_label /pred_at /= /usr_send_filter. naive_solver.
+Qed.
+
+Lemma retransmit_fair_traces_always_eventually_mAB (mtr : mtrace) :
+  usr_trace_valid mtr → usr_fair mtr →
+  (□ ◊ ℓ↓ usr_send_filter mAB) mtr.
+Proof.
+  intros Hvalid [Hfairn Hfairs]. eapply trace_always_implies_always_strong;
+    [|apply trace_always_and; split; [apply Hvalid|apply Hfairn]].
+  intros tr' Hsuff [Hvalid' Hfair']%trace_always_and.
+  apply retransmit_fair_traces_eventually_mAB=>//. split=>//.
+  - intros msg. eapply trace_always_suffix_of in Hfairn=>//.
+  - intros ρ. eapply trace_always_suffix_of in Hfairs=>//.
+  Unshelve. exact inhabitant.
+Qed.
 
 
 (* Lemma B_terminates (mtr : mtrace) : *)
@@ -308,21 +291,3 @@ Admitted.
 (*     inversion Hval; simplify_eq; try set_solver. } *)
 (*   rewrite /trace_now /pred_at /=. destruct mtr''=>//. *)
 (* Qed. *)
-
-
-Definition retransmit_lts : Lts (retransmit_role * option (action aneris_lang)) :=
-  {|
-            lts_state := retransmit_state;
-            lts_trans := retransmit_trans;
-  |}.
-
-Definition retransmit_model : UserModel aneris_lang.
-Proof.
-  refine({|
-            usr_role := retransmit_role;
-            usr_lts := retransmit_lts;
-            usr_live_roles := retransmit_live_roles;
-            usr_live_spec := retransmit_live_spec_holds;
-            usr_fl _ := 20;
-          |}).
-Defined.
